src/tls/MITLS.Repr.HSM13.fst
@@ -97,8 +97,8 @@ unfold let repr_post
     B.(modifies loc_none h0 h1) /\
     valid rr h1 /\  //the returned repr is valid in h1
     value r == f (value rr) /\  //relation between the values of the two reprs
-    r.start_pos <= rr.start_pos /\  //slice indices for the instance repr are contained in the slice indices of r
-    r.end_pos == rr.end_pos
+    r.start_pos <= rr.start_pos /\  //slice indices for the instance repr are contained in the slice indices of r ...
+    rr.end_pos <= r.end_pos  //... useful for framing
 
 let get_ee_repr (#b:R.slice) (r:repr b{is_ee r})
   : Stack (EERepr.repr b)
@@ -106,11 +106,9 @@ let get_ee_repr (#b:R.slice) (r:repr b{is_ee r})
     (ensures  repr_post r HSM13.M13_encrypted_extensions)
   = R.reveal_valid ();
     let ee_begin = HSM13.handshake13_accessor_encrypted_extensions b r.R.start_pos in
+    let ee_end = HSM13.handshake13_m13_encrypted_extensions_validator b ee_begin in
 
-    let h = ST.get () in
-    assume (v ee_begin + LP.content_length HSM13.handshake13_m13_encrypted_extensions_parser h b ee_begin == v r.R.end_pos);
-
-    R.mk b ee_begin r.R.end_pos HSM13.handshake13_m13_encrypted_extensions_parser
+    R.mk b ee_begin ee_end HSM13.handshake13_m13_encrypted_extensions_parser
 
 let get_c_repr (#b:R.slice) (r:repr b{is_c r})
   : Stack (CRepr.repr b)
@@ -118,23 +116,19 @@ let get_c_repr (#b:R.slice) (r:repr b{is_c r})
     (ensures  repr_post r HSM13.M13_certificate)
   = R.reveal_valid ();
     let c_begin = HSM13.handshake13_accessor_certificate b r.R.start_pos in
+    let c_end = HSM13.handshake13_m13_certificate_validator b c_begin in
     
-    let h = ST.get () in
-    assume (v c_begin + LP.content_length HSM13.handshake13_m13_certificate_parser h b c_begin == v r.R.end_pos);
-    
-    R.mk b c_begin r.R.end_pos HSM13.handshake13_m13_certificate_parser
+    R.mk b c_begin c_end HSM13.handshake13_m13_certificate_parser
 
 let get_cv_repr (#b:R.slice) (r:repr b{is_cv r})
   : Stack (CVRepr.repr b)
     (requires repr_pre r)
     (ensures  repr_post r HSM13.M13_certificate_verify)
   = R.reveal_valid ();
-    let c_begin = HSM13.handshake13_accessor_certificate_verify b r.R.start_pos in
-    
-    let h = ST.get () in
-    assume (v c_begin + LP.content_length HSM13.handshake13_m13_certificate_verify_parser h b c_begin == v r.R.end_pos);
-    
-    R.mk b c_begin r.R.end_pos HSM13.handshake13_m13_certificate_verify_parser
+    let cv_begin = HSM13.handshake13_accessor_certificate_verify b r.R.start_pos in
+    let cv_end = HSM13.handshake13_m13_certificate_verify_validator b cv_begin in
+
+    R.mk b cv_begin cv_end HSM13.handshake13_m13_certificate_verify_parser
 
 let get_fin_repr (#b:R.slice) (r:repr b{is_fin r})
   : Stack (FinRepr.repr b)
@@ -142,8 +136,6 @@ let get_fin_repr (#b:R.slice) (r:repr b{is_fin r})
     (ensures  repr_post r HSM13.M13_finished)
   = R.reveal_valid ();
     let f_begin = HSM13.handshake13_accessor_finished b r.R.start_pos in
+    let f_end = HSM13.handshake13_m13_finished_validator b f_begin in
     
-    let h = ST.get () in
-    assume (v f_begin + LP.content_length HSM13.handshake13_m13_finished_parser h b f_begin == v r.R.end_pos);
-    
-    R.mk b f_begin r.R.end_pos HSM13.handshake13_m13_finished_parser
+    R.mk b f_begin f_end HSM13.handshake13_m13_finished_parser
